start on pulling out useful typechecker... might have lots of admits

veric/expr.v
@@ -1052,133 +1052,6 @@ match t1, t2 with
 | _, _ => false
 end.
 
-
-(** Main typechecking function, with work will typecheck both pure
-and non-pure expressions, for now mostly just works with pure expressions **)
-Fixpoint typecheck_expr (Delta : tycontext) (e: expr) : tc_assert :=
-let tcr := typecheck_expr Delta in
-match e with
- | Econst_int _ (Tint I32 _ _) => tc_TT 
- | Econst_float _ (Tfloat F64 _) => tc_TT
- | Econst_single _ (Tfloat F32 _) => tc_TT
- | Etempvar id ty => 
-                       match (temp_types Delta)!id with 
-                         | Some ty' => if is_neutral_cast (fst ty') ty || same_base_type (fst ty') ty then 
-                                         if (snd ty') then tc_TT else (tc_initialized id ty)
-                                       else tc_FF (mismatch_context_type ty (fst ty'))
-		         | None => tc_FF (var_not_in_tycontext Delta id)
-                       end
- | Eaddrof a ty => tc_andp (typecheck_lvalue Delta a) (tc_bool (is_pointer_type ty)
-                                                      (op_result_type e))
- | Eunop op a ty => tc_andp (tc_bool (isUnOpResultType op a ty) (op_result_type e)) (tcr a)
- | Ebinop op a1 a2 ty => tc_andp (tc_andp (isBinOpResultType op a1 a2 ty)  (tcr a1)) (tcr a2)
- | Ecast a ty => tc_andp (tcr a) (isCastResultType (typeof a) ty a)
- | Evar id ty => match access_mode ty with
-                         | By_reference => 
-                            match get_var_type Delta id with 
-                            | Some ty' => tc_bool (eqb_type ty ty') 
-                                                           (mismatch_context_type ty ty') 
-                            | None => tc_FF (var_not_in_tycontext Delta id)
-                            end 
-                         | _ => tc_FF (deref_byvalue ty)
-                        end
- | Efield a i ty => match access_mode ty with
-                         | By_reference => 
-                            tc_andp (typecheck_lvalue Delta a) (match typeof a with
-                            | Tstruct id fList att =>
-                                  match field_offset i fList with 
-                                  | Errors.OK delta => tc_TT
-                                  | _ => tc_FF (invalid_struct_field i fList)
-                                  end
-                            | Tunion id fList att => tc_TT
-                            | _ => tc_FF (invalid_field_access e)
-                            end)
-                         | _ => tc_FF (deref_byvalue ty)
-                        end
- | Ederef a ty => match access_mode ty with
-                  | By_reference => tc_andp 
-                       (tc_andp 
-                          (typecheck_expr Delta a) 
-                          (tc_bool (is_pointer_type (typeof a))(op_result_type e)))
-                       (tc_isptr a)
-                  | _ => tc_FF (deref_byvalue ty)
-                  end
- | _ => tc_FF (invalid_expression e)
-end
-
-with typecheck_lvalue (Delta: tycontext) (e: expr) : tc_assert :=
-match e with
- | Evar id ty => match get_var_type Delta id with 
-                  | Some ty' => tc_bool (eqb_type ty ty') 
-                                           (mismatch_context_type ty ty')        
-                  | None => tc_FF (var_not_in_tycontext Delta id)
-                 end
- | Ederef a ty => tc_andp 
-                       (tc_andp 
-                          (typecheck_expr Delta a) 
-                          (tc_bool (is_pointer_type (typeof a))(op_result_type e)))
-                       (tc_isptr a)
- | Efield a i ty => tc_andp 
-                         (typecheck_lvalue Delta a) 
-                         (match typeof a with
-                            | Tstruct id fList att =>
-                              match field_offset i fList with 
-                                | Errors.OK delta => tc_TT
-                                | _ => tc_FF (invalid_struct_field i fList)
-                              end
-                            | Tunion id fList att => tc_TT
-                            | _ => tc_FF (invalid_field_access e)
-                          end)
- | _  => tc_FF (invalid_lvalue e)
-end.
-
-Definition implicit_deref (t: type) : type :=
-  match t with
-  | Tarray t' _ _ => Tpointer t' noattr
-  | _ => t
-  end.
-
-Definition typecheck_temp_id id ty Delta a : tc_assert :=
-  match (temp_types Delta)!id with
-  | Some (t,_) => 
-      tc_andp (tc_bool (is_neutral_cast (implicit_deref ty) t) (invalid_cast ty t)) 
-                  (isCastResultType (implicit_deref ty) t a)
-  | None => tc_FF (var_not_in_tycontext Delta id)
- end.
-
-Fixpoint tc_might_be_true (asn : tc_assert) :=
-match asn with
- | tc_FF _ => false
- | tc_andp' a1 a2 => tc_might_be_true a1 && tc_might_be_true a2
- | _ => true
-end.
-
-Fixpoint tc_always_true (asn : tc_assert) := 
-match asn with
- | tc_TT => true
- | tc_andp' a1 a2 => tc_always_true a1 && tc_always_true a2
- | _ => false
-end.
-
-
-
-(* A more standard typechecker, should approximate the c typechecker,
-might need to add a tc_noproof for nested loads*)
-Definition typecheck_b Delta e :=  tc_might_be_true (typecheck_expr Delta e).
-
-(*Definition of the original *pure* typechecker where true means the expression
-will always evaluate, may not be useful since tc_denote will just compute to true
-on these assertions*)
-Definition typecheck_pure_b Delta e := tc_always_true (typecheck_expr Delta e). 
-
-Fixpoint typecheck_exprlist (Delta : tycontext) (tl : list type) (el : list expr) : tc_assert :=
-match tl,el with
-| t::tl', e:: el' => tc_andp (typecheck_expr Delta (Ecast e t)) 
-                      (typecheck_exprlist Delta tl' el')
-| nil, nil => tc_TT
-| _, _ => tc_FF wrong_signature
-end.
-
 Definition typecheck_val (v: val) (ty: type) : bool :=
  match v, ty with
  | Vint i, Tint sz sg _ => 
@@ -1216,6 +1089,64 @@ Fixpoint typecheck_vals (v: list val) (ty: list type) : bool :=
  | nil, nil => true
  | _, _ => false
 end.
+
+
+(** Main typechecking function, with work will typecheck both pure
+and non-pure expressions, for now mostly just works with pure expressions **)
+Definition typecheck_expr (Delta : tycontext) (e : expr)  :  environ -> Prop :=
+  `eq (`typecheck_val (eval_expr e ) `(typeof e)) `true.
+
+Definition typecheck_lvalue (Delta: tycontext) e  : environ -> Prop :=
+fun rho => (             
+             typecheck_val (eval_lvalue e rho) (typeof e) = true).
+
+
+
+Definition implicit_deref (t: type) : type :=
+  match t with
+  | Tarray t' _ _ => Tpointer t' noattr
+  | _ => t
+  end.
+
+Definition typecheck_temp_id id ty Delta a : tc_assert :=
+  match (temp_types Delta)!id with
+  | Some (t,_) => 
+      tc_andp (tc_bool (is_neutral_cast (implicit_deref ty) t) (invalid_cast ty t)) 
+                  (isCastResultType (implicit_deref ty) t a)
+  | None => tc_FF (var_not_in_tycontext Delta id)
+ end.
+
+Fixpoint tc_might_be_true (asn : tc_assert) :=
+match asn with
+ | tc_FF _ => false
+ | tc_andp' a1 a2 => tc_might_be_true a1 && tc_might_be_true a2
+ | _ => true
+end.
+
+Fixpoint tc_always_true (asn : tc_assert) := 
+match asn with
+ | tc_TT => true
+ | tc_andp' a1 a2 => tc_always_true a1 && tc_always_true a2
+ | _ => false
+end.
+
+
+
+(* A more standard typechecker, should approximate the c typechecker,
+might need to add a tc_noproof for nested loads*)
+
+(*Definition of the original *pure* typechecker where true means the expression
+will always evaluate, may not be useful since tc_denote will just compute to true
+on these assertions*)
+
+Fixpoint typecheck_exprlist (Delta : tycontext) (tl : list type) (el : list expr) : environ -> Prop :=
+match tl,el with
+| t::tl', e:: el' => `and (typecheck_expr Delta (Ecast e t)) 
+                      (typecheck_exprlist Delta tl' el')
+| nil, nil => `True
+| _, _ => `False
+end.
+
 
 
 (** Environment typechecking functions **)
@@ -1269,105 +1200,6 @@ typecheck_var_environ  (ve_of rho) (var_types Delta) /\
 typecheck_glob_environ (ge_of rho) (glob_types Delta) /\
 same_env rho Delta.
 
-(** Denotation functions for each of the assertions that can be produced by the typechecker **)
-
-Definition denote_tc_iszero v :=
-         match v with Vint i => is_true (Int.eq i Int.zero) 
-                            | Vlong i => is_true (Int.eq (Int.repr (Int64.unsigned i)) Int.zero)
-                            | _ => False 
-         end.
-
-Definition denote_tc_nonzero v := 
-         match v with Vint i => if negb (Int.eq i Int.zero) then True else False
-                                               | _ => False end.
-
-Definition denote_tc_igt i v :=
-     match v with | Vint i1 => is_true (Int.ltu i1 i)
-                     | _ => False
-                  end.
-
-Definition Zoffloat (f:float): option Z := (**r conversion to Z *)
-  match f with
-    | Fappli_IEEE.B754_finite s m (Zpos e) _ => 
-       Some (Fcore_Zaux.cond_Zopp s (Zpos m) * Zpower_pos 2 e)
-    | Fappli_IEEE.B754_finite s m 0 _ => Some (Fcore_Zaux.cond_Zopp s (Zpos m))
-    | Fappli_IEEE.B754_finite s m (Zneg e) _ => Some (Fcore_Zaux.cond_Zopp s (Zpos m / Zpower_pos 2 e))
-    | Fappli_IEEE.B754_zero _ => Some 0
-    | _ => None
-  end.  (* copied from CompCert 2.3, because it's missing in CompCert 2.4 *)
-
-Definition Zofsingle (f: float32): option Z := (**r conversion to Z *)
-  match f with
-    | Fappli_IEEE.B754_finite s m (Zpos e) _ => 
-       Some (Fcore_Zaux.cond_Zopp s (Zpos m) * Zpower_pos 2 e)
-    | Fappli_IEEE.B754_finite s m 0 _ => Some (Fcore_Zaux.cond_Zopp s (Zpos m))
-    | Fappli_IEEE.B754_finite s m (Zneg e) _ => Some (Fcore_Zaux.cond_Zopp s (Zpos m / Zpower_pos 2 e))
-    | Fappli_IEEE.B754_zero _ => Some 0
-    | _ => None
-  end.  (* copied from CompCert 2.3, because it's missing in CompCert 2.4 *)
-
-
-Definition denote_tc_Zge z v := 
-          match v with
-                     | Vfloat f => match Zoffloat f with
-                                    | Some n => is_true (Zge_bool z n)
-                                    | None => False
-                                   end
-                     | Vsingle f => match Zofsingle f with
-                                    | Some n => is_true (Zge_bool z n)
-                                    | None => False
-                                   end
-                     | _ => False 
-                  end.
-
-Definition denote_tc_Zle z v := 
-          match v with
-                     | Vfloat f => match Zoffloat f with
-                                    | Some n => is_true (Zle_bool z n)
-                                    | None => False
-                                   end
-                     | Vsingle f => match Zofsingle f with
-                                    | Some n => is_true (Zle_bool z n)
-                                    | None => False
-                                   end
-                     | _ => False 
-                  end.
-
-Definition denote_tc_samebase v1 v2 :=
-                         match v1, v2 with
-                           | Vptr b1 _, Vptr b2 _ => is_true (peq b1 b2)
-                           | _, _ => False 
-                         end.
-
-(** Case for division of int min by -1, which would cause overflow **)
-Definition denote_tc_nodivover v1 v2 :=
-match v1, v2 with
-                           | Vint n1, Vint n2 => is_true (negb 
-                                   (Int.eq n1 (Int.repr Int.min_signed) 
-                                    && Int.eq n2 Int.mone))
-                           | _ , _ => False
-                          end.
-
-Definition denote_tc_initialized id ty rho := exists v, Map.get (te_of rho) id = Some v
-                                            /\ is_true (typecheck_val v ty).
-
-Fixpoint denote_tc_assert (a: tc_assert) : environ -> Prop :=
-  match a with
-  | tc_FF _ => `False
-  | tc_noproof => `False
-  | tc_TT => `True
-  | tc_andp' b c => `and (denote_tc_assert b) (denote_tc_assert c)
-  | tc_orp' b c => `or (denote_tc_assert b) (denote_tc_assert c)
-  | tc_nonzero' e => `denote_tc_nonzero (eval_expr e)
-  | tc_isptr e => `isptr (eval_expr e)
-  | tc_ilt' e i => `(denote_tc_igt i) (eval_expr e)
-  | tc_Zle e z => `(denote_tc_Zge z) (eval_expr e)
-  | tc_Zge e z => `(denote_tc_Zle z) (eval_expr e)
-  | tc_samebase e1 e2 => `denote_tc_samebase (eval_expr e1) (eval_expr e2)
-  | tc_nodivover' v1 v2 => `denote_tc_nodivover (eval_expr v1) (eval_expr v2)
-  | tc_initialized id ty => denote_tc_initialized id ty
-  | tc_iszero' e => `denote_tc_iszero (eval_expr e)
- end.
 
 Lemma and_False: forall x, (x /\ False) = False.
 Proof.
@@ -1390,25 +1222,6 @@ intros; apply prop_ext; intuition.
 Qed.
 
 
-Lemma tc_andp_sound : forall a1 a2 rho, denote_tc_assert (tc_andp a1 a2) rho <->  denote_tc_assert (tc_andp' a1 a2) rho. 
-Proof.
-intros.
- unfold tc_andp.
- destruct a1; simpl; unfold_lift;
- repeat first [rewrite False_and | rewrite True_and | rewrite and_False | rewrite and_True];
-  try apply iff_refl;
-  destruct a2; simpl in *; unfold_lift;
- repeat first [rewrite False_and | rewrite True_and | rewrite and_False | rewrite and_True];
-  try apply iff_refl.
-Qed. 
-
-Lemma denote_tc_assert_andp: 
-  forall a b rho, denote_tc_assert (tc_andp a b) rho =
-             (denote_tc_assert a rho /\ denote_tc_assert b rho).
-Proof.
- intros. apply prop_ext. rewrite tc_andp_sound.
- simpl; apply iff_refl.
-Qed.
 
 (** Functions that modify type environments **)
 Definition initialized id (Delta: tycontext) : tycontext :=
@@ -1752,102 +1565,10 @@ Lemma tc_val_eq':
   forall t v, (typecheck_val v t = true) =  tc_val t v.
 Proof. intros. rewrite tc_val_eq. auto. Qed.
 
-Lemma neutral_isCastResultType:
-  forall t t' v rho,
-   is_neutral_cast t' t = true ->
-   denote_tc_assert (isCastResultType t' t v) rho.
-Proof.
-intros.
-  unfold isCastResultType;
-  destruct t'  as [ | [ | | | ] [ | ] | | [ | ] | | | | | | ], t  as [ | [ | | | ] [ | ] | | [ | ] | | | | | | ];
-     inv H; try apply I;
-    simpl; if_tac; apply I.
-Qed.
+Definition denote_tc_assert (a : environ -> Prop) := 
+a. 
 
 (*A boolean denote_tc_assert *)
-
-Definition denote_tc_iszero_b v :=
-         match v with Vint i => (Int.eq i Int.zero) 
-                            | Vlong i =>  (Int.eq (Int.repr (Int64.unsigned i)) Int.zero)
-                            | _ => false 
-         end.
-
-Definition denote_tc_nonzero_b v := 
-         match v with Vint i => if negb (Int.eq i Int.zero) then true else false
-                                               | _ => false end.
-
-Definition denote_tc_igt_b i v :=
-     match v with | Vint i1 => (Int.ltu i1 i)
-                     | _ => false
-                  end.
-
-Definition denote_tc_Zge_b z v := 
-          match v with
-                     | Vfloat f => match Zoffloat f with
-                                    | Some n => (Zge_bool z n)
-                                    | None => false
-                                   end
-                     | Vsingle f => match Zofsingle f with
-                                    | Some n => (Zge_bool z n)
-                                    | None => false
-                                   end
-                     | _ => false 
-                  end.
-
-Definition denote_tc_Zle_b z v := 
-          match v with
-                     | Vfloat f => match Zoffloat f with
-                                    | Some n => (Zle_bool z n)
-                                    | None => false
-                                   end
-                     | Vsingle f => match Zofsingle f with
-                                    | Some n => (Zle_bool z n)
-                                    | None => false
-                                   end
-                     | _ => false 
-                  end.
-
-Definition denote_tc_samebase_b v1 v2 :=
-                         match v1, v2 with
-                           | Vptr b1 _, Vptr b2 _ => (peq b1 b2)
-                           | _, _ => false 
-                         end.
-
-(** Case for division of int min by -1, which would cause overflow **)
-Definition denote_tc_nodivover_b v1 v2 :=
-match v1, v2 with
-                           | Vint n1, Vint n2 => (negb 
-                                   (Int.eq n1 (Int.repr Int.min_signed) 
-                                    && Int.eq n2 Int.mone))
-                           | _ , _ => false
-                          end.
-
-Definition denote_tc_initialized_b id ty rho := 
-match Map.get (te_of rho) id with 
-| Some v => typecheck_val v ty
-| None => false
-end.
-
-Definition isptr_b v := 
-   match v with | Vptr _ _ => true | _ => false end.
-
-Fixpoint denote_tc_assert_b (a: tc_assert) : environ -> bool :=
-  match a with
-  | tc_FF _ => `false
-  | tc_noproof => `false
-  | tc_TT => `true
-  | tc_andp' b c => `andb (denote_tc_assert_b b) (denote_tc_assert_b c)
-  | tc_orp' b c => `orb (denote_tc_assert_b b) (denote_tc_assert_b c)
-  | tc_nonzero' e => `denote_tc_nonzero_b (eval_expr e)
-  | tc_isptr e => `isptr_b (eval_expr e)
-  | tc_ilt' e i => `(denote_tc_igt_b i) (eval_expr e)
-  | tc_Zle e z => `(denote_tc_Zge_b z) (eval_expr e)
-  | tc_Zge e z => `(denote_tc_Zle_b z) (eval_expr e)
-  | tc_samebase e1 e2 => `denote_tc_samebase_b (eval_expr e1) (eval_expr e2)
-  | tc_nodivover' v1 v2 => `denote_tc_nodivover_b (eval_expr v1) (eval_expr v2)
-  | tc_initialized id ty => denote_tc_initialized_b id ty
-  | tc_iszero' e => `denote_tc_iszero_b (eval_expr e)
- end.
 
 Lemma false_true : False <-> false=true.
 intuition.
@@ -1894,58 +1615,3 @@ bool_n H.
 Tactic Notation "bool_r" "in" "*" :=
 bool_s.
 
-Definition denote_te_assert_b_eq : forall a rho, 
-denote_tc_assert a rho <-> is_true (denote_tc_assert_b a rho).
-Proof. intros. split; intros.
-induction a; simpl in *; super_unfold_lift; bool_r in *; intuition;
-simpl in *;
-try destruct (eval_expr e); simpl in *;
-try match goal with 
-| [ H : if ?e then True else False |- _ ] => destruct e; simpl; inv H
-| [ H : match ?e with | _ => _  end |- _ ] => destruct e; simpl in *; inv H
-end; auto; try congruence;
-unfold denote_tc_initialized, denote_tc_initialized_b in *.
-destruct (denote_tc_assert_b a1 rho); try contradiction; apply I.
-destruct (denote_tc_assert_b a1 rho); try contradiction; apply I.
-destruct (Zoffloat f); try contradiction.
-destruct (z >=? z0); try contradiction; auto.
-destruct (Zofsingle f); try contradiction.
-destruct (z >=? z0); try contradiction; auto.
-destruct (Zoffloat f); try contradiction.
-destruct (z <=? z0); try contradiction; auto.
-destruct (Zofsingle f); try contradiction.
-destruct (z <=? z0); try contradiction; auto.
-destruct (eval_expr e0 rho); try contradiction.
-destruct (peq b b0); try contradiction; auto.
-destruct (eval_expr e0 rho); try contradiction.
-destruct (negb (Int.eq i (Int.repr Int.min_signed) && Int.eq i0 Int.mone)); try contradiction; auto.
-destruct H. destruct H; rewrite H. auto.
-
-induction a; simpl in *; super_unfold_lift; bool_r in *; intuition; try congruence;
-simpl in *;
-try destruct (eval_expr e); simpl in *; try congruence;
-try match goal with 
-| [ H : (if ?e then true else false) = true |- _ ] => destruct e; simpl; inv H
-| [ H : (match ?e with | _ => _ end) = true |- _ ] => destruct e; simpl in *; inv H
-end; auto; try congruence.
-unfold denote_tc_initialized, denote_tc_initialized_b in *.
-destruct (denote_tc_assert_b a1 rho); try contradiction; auto.
-destruct (denote_tc_assert_b a1 rho); try contradiction; auto.
-destruct (denote_tc_assert_b a1 rho); try contradiction; auto.
-destruct (negb (Int.eq i Int.zero)); try contradiction; auto.
-destruct (Zoffloat f); try contradiction.
-destruct (z >=? z0); try contradiction; auto.
-destruct (Zofsingle f); try contradiction.
-destruct (z >=? z0); try contradiction; auto.
-destruct (Zoffloat f); try contradiction.
-destruct (z <=? z0); try contradiction; auto.
-destruct (Zofsingle f); try contradiction.
-destruct (z <=? z0); try contradiction; auto.
-destruct (eval_expr e0 rho); try contradiction.
-destruct (peq b b0); try contradiction; auto.
-destruct (eval_expr e0 rho); try contradiction.
-destruct (negb (Int.eq i (Int.repr Int.min_signed) && Int.eq i0 Int.mone)); try contradiction; auto.
-unfold denote_tc_initialized_b in H.
-destruct (Map.get (te_of rho) e) eqn:?; try contradiction.
-exists v; split; auto.
-Qed.
